dsada

proj/proj_verify/weight_calculation.dfy
@@ -87,14 +87,17 @@ method findMin(a:array?<real>) returns(min:real)
 
 }
 
-method scoreSum(){
+method Main() returns (sums array<int>)
+ensure forall i:: 0 <= i < bloods.length sums[i] == calc
+{
 
-//  var bloods: array<real> := new real[5];
-//  bloods[0],bloods[1],bloods[2],bloods[3],bloods[4] := 10.0 ,8.0, 15.0, 17.0, 7.0;
+  var bloods: array<real> := new real[5];
+  bloods[0],bloods[1],bloods[2],bloods[3],bloods[4] := 10.0 ,8.0, 15.0, 17.0, 7.0;
 
-//  var min := findMin(bloods);
+  var min := findMin(bloods);
 //  //print(min);
-//  //assert min == 7.0;
+  assert (bloods[4] < bloods[1] < bloods[0] < bloods[2] < bloods[3]);
+  assert min == 7.0;
 //  var max := findMax(bloods);
 //  //print(max);
 //  //assert max == 17.0;
@@ -146,7 +149,6 @@ method scoreSum(){
     i := i + 1;
   }
   /////////////////////////////////
-
   i := 0;
   while i < scores.Length
   invariant 0 <= i <= scores.Length
@@ -166,4 +168,200 @@ method scoreSum(){
   /////////////////////////////////
 
   //print(scores[..]);
+}
+https://rise4fun.com/Dafny/JOOTh
+
+
+//method scoreSum() //returns (sums: array<real>)
+////ensures forall i :: 0 <= i < bloods.Length ==> sums[i] == calc
+//{
+// scores
+//}
+//  var bloods: array<real> := new real[5];
+//  bloods[0],bloods[1],bloods[2],bloods[3],bloods[4] := 10.0 ,8.0, 15.0, 17.0, 7.0;
+//
+//  var min := findMin(bloods);
+//  assert (bloods[4] < bloods[1] < bloods[0] < bloods[2] < bloods[3]);
+//  assert min == 7.0;
+//  var max := findMax(bloods);
+//  assert (bloods[3] > bloods[2] > bloods[0] > bloods[1] > bloods[4]);
+//  assert max == 17.0;
+//
+//  var weightage: array<real> := new real[4];
+//  weightage[0],weightage[1],weightage[2],weightage[3] := 0.52, 0.27, -0.15, 0.06;
+//
+//  var expiry: array<real> := new real[4];
+//  expiry[0],expiry[1],expiry[2],expiry[3] := 3.0 ,5.0, 8.0, 1.0;
+//
+//calScore(expiry, w[0])
+//  var minE := findMin(expiry);
+//  var maxE := findMax(expiry);
+//
+//  var quantity: array<real> := new real[4];
+//  quantity[0],quantity[1],quantity[2],quantity[3] := 50.0 ,60.0, 20.0, 70.0;
+//
+//  var minQ := findMin(quantity);
+//  var maxQ := findMax(quantity);
+//
+//  var rank: array<real> := new real[4];
+//  rank[0],rank[1],rank[2],rank[3] := 7.0, 5.0, 2.0, 1.0;
+//
+//  var minR := findMin(rank);
+//  var maxR := findMax(rank);
+//
+//  var totalQ: array<real> := new real[4];
+//  totalQ[0],totalQ[1],totalQ[2],totalQ[3] := 800.0 ,750.0, 1000.0, 800.0;
+//
+//  var minT := findMin(totalQ);
+//  var maxT := findMax(totalQ);
+//
+//  var scores: array<real> := new real[expiry.Length];
+//  assert (scores.Length == expiry.Length);
+//
+//  var i := 0;
+//  while i < scores.Length
+//  invariant 0 <= i <= scores.Length
+//  {
+//    scores[i] := scores[i] + calcScore(expiry[i], minE, maxE, weightage[0]);
+//    i := i + 1;
+//  }
+//  /////////////////////////////////
+//
+//  i := 0;
+//  while i < scores.Length
+//  invariant 0 <= i <= scores.Length
+//  {
+//    scores[i] := scores[i] + calcScore(quantity[i], minQ, maxQ, weightage[1]);
+//    i := i + 1;
+//  }
+//  /////////////////////////////////
+//
+//  i := 0;
+//  while i < scores.Length
+//  invariant 0 <= i <= scores.Length
+//  {
+//    scores[i] := scores[i] + calcScore(rank[i], minR, maxR, weightage[2]);
+//    i := i + 1;
+//  }
+//  /////////////////////////////////
+//
+//  i := 0;
+//  while i < scores.Length
+//  invariant 0 <= i <= scores.Length
+//  {
+//    scores[i] := scores[i] + calcScore(totalQ[i], minT, maxT, weightage[3]);
+//    i := i + 1;
+//  }
+//  /////////////////////////////////
+//
+//  //print(scores[..]);
+//}
+
+// predicate to make sure the blood weight are initialise to zero
+// TODO change int to BLOOD datatype
+predicate bloodZero(bloods: array?<int>)
+  reads bloods
+  requires bloods != null
+{
+  forall b :: 0 <= b < bloods.Length ==> bloods[b] == 0
+}
+
+// calculate score from given parameter
+function method calcScore(value:real , min:real , max:real, weight:real ) : real
+requires max != 0.0
+{
+  if weight > 0.0
+    then weight *( 1.0- (value-min) / max )
+  else
+    weight * (( value-min) / max )
+}
+// find maximum value for the given array of criteria value
+method findMax(a:array?<real>) returns(max:real)
+ requires a!=null;
+ ensures (forall j :int :: (j >= 0 && j < a.Length ==> max >= a[j]));
+ ensures (a.Length > 0)==>(exists j : int :: j>=0 && j < a.Length && max==a[j]);
+{
+  if (a.Length == 0)
+  {
+    max := 0.0;
+  }
+  else
+  {
+    max:=a[0];
+    var i:int :=1;
+
+    while(i < a.Length)
+    invariant (i<=a.Length)
+    invariant (forall j:int :: j>=0 && j<i ==> max >= a[j]);
+    invariant (exists j:int :: j>=0 && j<i && max==a[j]);
+    decreases (a.Length-i);
+    {
+
+     if(a[i] > max)
+     {
+       max := a[i];
+     }
+
+     i := i + 1;
+
+    }
+  }
+
+}
+
+
+method findMin(a:array?<real>) returns(min:real)
+ requires a!=null;
+ ensures (forall j :int :: (j >= 0 && j < a.Length ==> min <= a[j]));
+ ensures (a.Length > 0)==>(exists j : int :: j>=0 && j < a.Length && min==a[j]);
+{
+  if (a.Length == 0)
+  {
+    min := 0.0;
+  }
+  else
+  {
+    min:=a[0];
+    var i:int :=1;
+
+    while(i < a.Length)
+    invariant (i<=a.Length)
+    invariant (forall j:int :: j>=0 && j<i ==> min <= a[j]);
+    invariant (exists j:int :: j>=0 && j<i && min==a[j]);
+    decreases (a.Length-i);
+    {
+
+     if(a[i] < min)
+     {
+       min := a[i];
+     }
+
+     i := i + 1;
+
+    }
+  }
+
+}
+
+method calcScoreForEachCriteria(criteria: array<real>, w:real) returns (scores: array<real>)
+//ensures
+//requires criteria.Length == scores.Length
+{
+//  var totalQ: array<real> := new real[4];
+//  totalQ[0],totalQ[1],totalQ[2],totalQ[3] := 800.0 ,750.0, 1000.0, 800.0;
+  scores := new real[criteria.Length];
+  var min := findMin(criteria);
+  var max := findMax(criteria);
+
+//  var scores: array<real> := new real[expiry.Length];
+//  assert (scores.Length == expiry.Length);
+
+  var i := 0;
+  while i < criteria.Length
+  invariant 0 <= i <= criteria.Length
+  {
+    scores[i] := scores[i] + calcScore(criteria[i], min, max, w);
+    i := i + 1;
+  }
+
 }
